attempt to prove things about the shol semantics
first tried proving that the semantics of a term is a member of the
semantics of its type. this led to wanting to prove that the semantics
relation is functional (it won't be total, though). this led to various
tweaks to the semantics definition and also to the inference system -
requiring various terms to be welltyped and closed etc. still not
proved. the difficulty now is to show:

if INST tyin t and INST tyin' t have the same type, and the type
variables in t all appear in the type of t, then in fact INST tyin t =
INST tyin' t. intuitively, type instantiation only instantiates type
variables, and since the result types are equal and all the type
variables are in the original type, they must have been instantiated the
same way. but this means another proof about INST_CORE whose definition
is complicated because of checking for accidental variable capture...

hol-light/sholSemanticsScript.sml
@@ -1,4 +1,4 @@
-open HolKernel boolLib bossLib lcsymtacs listTheory sholSyntaxTheory modelSetTheory
+open HolKernel boolLib bossLib lcsymtacs pred_setTheory listTheory finite_mapTheory sholSyntaxTheory modelSetTheory
 val _ = numLib.prefer_num()
 val _ = new_theory"sholSemantics"
 
@@ -36,9 +36,10 @@ val (semantics_rules,semantics_ind,semantics_cases) = Hol_reln`
        (λp. let mp = (mty suchthat holds p) in
             ch (if ∃x. x <: mp then mp else mty)))) ∧
 
-  (t has_type tyt ∧
-   TYPE_SUBST tyin tyt = ty ∧
-   semantics σ τ (INST tyin t) mt
+  (welltyped t ∧ closed t ∧
+   set(tvars t) ⊆ set (tyvars (typeof t)) ∧
+   INST tyin t has_type ty ∧
+   semantics FEMPTY τ (INST tyin t) mt
    ⇒
    semantics σ τ (Const s ty (Defined t)) mt) ∧
 
@@ -50,8 +51,8 @@ val (semantics_rules,semantics_ind,semantics_cases) = Hol_reln`
 
   (typeset τ rty mrty ∧
    typeset τ atr maty ∧
-   p has_type (Fun rtyp Bool) ∧
-   TYPE_SUBST tyin rtyp = rty ∧
+   welltyped p ∧ closed p ∧
+   INST tyin p has_type Fun rty Bool ∧
    semantics FEMPTY τ (INST tyin p) mp
    ⇒
    semantics σ τ (Const s (Fun rty aty) (Tyabs op p))
@@ -68,5 +69,177 @@ val (semantics_rules,semantics_ind,semantics_cases) = Hol_reln`
    (∀x. semantics (σ |+ ((n,ty),x)) τ b (mb x))
    ⇒
    semantics σ τ (Abs n ty b) (abstract mty mtyb mb))`
+
+val type_valuation_def = Define`
+  type_valuation τ ⇔ ∀x. ∃y. y <: τ x`
+
+val term_valuation_def = Define`
+  term_valuation τ σ ⇔
+    FEVERY (λ(v,m). ∀mty. typeset τ (SND v) mty ⇒ m <: mty) σ`
+
+val _ = Parse.add_infix("|=",450,Parse.NONASSOC)
+
+val sequent_def = xDefine"sequent"`
+  h |= c ⇔ EVERY (λt. t has_type Bool) (c::h) ∧
+           ∀σ τ. type_valuation τ ∧
+                 term_valuation τ σ ∧
+                 EVERY (λt. semantics σ τ t true) h
+                 ⇒
+                 semantics σ τ c true`
+
+val term_valuation_FUPDATE = store_thm("term_valuation_FUPDATE",
+  ``∀τ σ v m.
+    term_valuation τ σ ∧
+    (∀mty. typeset τ (SND v) mty ⇒ m <: mty)
+    ⇒
+    term_valuation τ (σ |+ (v,m))``,
+  rw[term_valuation_def,FEVERY_DEF,FAPPLY_FUPDATE_THM]>>PROVE_TAC[])
+
+val semantics_closed = store_thm("semantics_closed",
+  ``∀t σ τ mt. semantics σ τ t mt ⇒
+      ∀n ty. VFREE_IN (Var n ty) t ⇒ (n,ty) ∈ FDOM σ``,
+  reverse Induct >- (
+    simp[Once semantics_cases] >>
+    rpt gen_tac >> strip_tac >>
+    simp[CONJ_SYM] >>
+    simp[GSYM AND_IMP_INTRO] >>
+    rpt gen_tac >> strip_tac >>
+    `(n,ty) ∈ FDOM (σ |+ ((s,t),x))` by PROVE_TAC[] >>
+    fs[] ) >>
+  simp[Once semantics_cases] >>
+  simp[FLOOKUP_DEF] >>
+  metis_tac[])
+
+val type_ind =
+  TypeBase.induction_of``:type``
+  |> Q.SPECL[`K T`,`P`,`K T`,`K T`,`EVERY P`]
+  |> SIMP_RULE std_ss [EVERY_DEF]
+  |> UNDISCH_ALL
+  |> CONJUNCT1
+  |> DISCH_ALL
+  |> Q.GEN`P`
+
+val MEM_LIST_INSERT = store_thm("MEM_LIST_INSERT",
+  ``∀l x. set (LIST_INSERT x l) = x INSERT set l``,
+  Induct >> simp[LIST_INSERT_def] >> rw[] >>
+  rw[EXTENSION] >> metis_tac[])
+
+val MEM_LIST_UNION = store_thm("MEM_LIST_UNION",
+  ``∀l1 l2. set (LIST_UNION l1 l2) = set l1 ∪ set l2``,
+  Induct >> fs[LIST_UNION_def,MEM_LIST_INSERT] >>
+  rw[EXTENSION] >> metis_tac[])
+
+val TYPE_SUBST_tyvars = store_thm("TYPE_SUBST_tyvars",
+  ``∀ty tyin tyin'.
+    (TYPE_SUBST tyin ty = TYPE_SUBST tyin' ty) ⇔
+    ∀x. MEM x (tyvars ty) ⇒
+        REV_ASSOCD (Tyvar x) tyin' (Tyvar x) =
+        REV_ASSOCD (Tyvar x) tyin  (Tyvar x)``,
+  ho_match_mp_tac type_ind >>
+  simp[tyvars_def] >>
+  conj_tac >- metis_tac[] >>
+  Induct >> simp[] >>
+  gen_tac >> strip_tac >> fs[] >>
+  rpt gen_tac >> EQ_TAC >> strip_tac >> fs[] >>
+  fs[MEM_LIST_UNION] >> metis_tac[])
+
+(*
+val INST_CORE_tvars = store_thm("INST_CORE_tvars",
+  ``∀t env tyin tyin'.
+    (∀x. MEM x (tvars t) ⇒
+         REV_ASSOCD (Tyvar x) tyin' (Tyvar x) =
+         REV_ASSOCD (Tyvar x) tyin  (Tyvar x))
+    ⇒
+    INST_CORE env tyin t = INST_CORE env tyin' t``,
+  Induct >- (
+    simp[INST_CORE_def] >>
+    rw[]
+  ho_match_mp_tac term_ind
+
+val semantics_11 = store_thm("semantics_11",
+  ``(∀τ ty mty. typeset τ ty mty ⇒
+        ∀mty'. typeset τ ty mty' ⇒ mty' = mty) ∧
+    (∀σ τ t mt. semantics σ τ t mt ⇒
+        ∀mt'. semantics σ τ t mt' ⇒ mt' = mt)``,
+  ho_match_mp_tac semantics_ind >>
+  conj_tac >- simp[Once semantics_cases] >>
+  conj_tac >- simp[Once semantics_cases] >>
+  conj_tac >- (
+    rpt gen_tac >> strip_tac >>
+    simp[Once semantics_cases] >>
+    PROVE_TAC[] ) >>
+  conj_tac >- (
+    rpt gen_tac >> strip_tac >>
+    simp[Once semantics_cases] >> rw[] >>
+    `Fun ty Bool = Fun rty Bool` by (
+      metis_tac[WELLTYPED_LEMMA] ) >>
+    fs[] ) >>
+  conj_tac >- simp[Once semantics_cases] >>
+  conj_tac >- (
+    rpt gen_tac >> strip_tac >>
+    simp[Once semantics_cases] >> rw[] >> rw[]) >>
+  conj_tac >- (
+    rpt gen_tac >> strip_tac >>
+    simp[Once semantics_cases] >> rw[] >> rw[]) >>
+  conj_tac >- (
+    rpt gen_tac >> strip_tac >>
+    simp[Once semantics_cases] >> rw[] >> rw[] >>
+    qspecl_then[`sizeof t`,`t`,`[]`,`tyin`]mp_tac INST_CORE_HAS_TYPE >>
+    qspecl_then[`sizeof t`,`t`,`[]`,`tyin'`]mp_tac INST_CORE_HAS_TYPE >>
+    simp[] >> ntac 2 strip_tac >> fs[INST_def] >>
+    imp_res_tac WELLTYPED_LEMMA >> rw[] >> fs[]
+
+    `tyt' = tyt` by metis_tac[WELLTYPED_LEMMA] >> rw[] >>
+    TYPE_SUBST
+    print_find"TYPE_SUBST"
+
+    ) >>
+
+
+val semantics_typeset = store_thm("semantics_typeset",
+  ``∀tm ty. tm has_type ty ⇒
+      ∀σ τ mtm mty. type_valuation τ ∧ term_valuation τ σ ∧
+                    typeset τ ty mty ∧ semantics σ τ tm mtm
+                    ⇒ mtm <: mty``,
+  ho_match_mp_tac has_type_strongind >>
+  conj_tac >- (
+    simp[Once (CONJUNCT2 semantics_cases)] >>
+    rw[term_valuation_def] >>
+    imp_res_tac FEVERY_FLOOKUP >> fs[]) >>
+  conj_tac >- (
+    rpt gen_tac >> strip_tac >>
+    pop_assum mp_tac >>
+    simp[Once (CONJUNCT2 semantics_cases)] >>
+    rw[] >- (
+      qpat_assum`typeset τ (Fun X Y) Z`mp_tac >>
+      simp[Once (CONJUNCT1 semantics_cases)] >> strip_tac >>
+      qpat_assum`typeset τ (Fun X Y) Z`mp_tac >>
+      simp[Once (CONJUNCT1 semantics_cases)] >> strip_tac >>
+      pop_assum mp_tac >>
+      simp[Once (CONJUNCT1 semantics_cases)] >> strip_tac >>
+      rpt BasicProvers.VAR_EQ_TAC >>
+      match_mp_tac ABSTRACT_IN_FUNSPACE
+
+      print_apropos``x <: funspace y z``
+
+
+val semantics_typeset = store_thm("semantics_typeset",
+  ``(∀τ ty mty. typeset τ ty mty ⇒
+        ∀σ t mt. type_valuation τ ∧ term_valuation τ σ ∧
+                 t has_type ty ∧ semantics σ τ t mt ⇒
+                 mt <: mty) ∧
+    (∀σ τ t mt. semantics σ τ t mt ⇒
+        ∀ty mty. type_valuation τ ∧ term_valuation τ σ ∧
+                 t has_type ty ∧ typeset τ ty mty ⇒
+                 mt <: mty)``,
+
+  ho_match_mp_tac semantics_ind >>
+  simp[INDSET_INHABITED,FUNSPACE_INHABITED] >>
+  conj_tac >- simp[type_valuation_def] >>
+  conj_tac >- metis_tac[BOOLEAN_IN_BOOLSET] >>
+
+  gen_tac >> Induct >> simp[Once semantics_cases]
+  Induct
+*)
 
 val _ = export_theory()
